theories/type_preservation.v
@@ -16,20 +16,9 @@ Variable host_function : eqType.
 
 Let store_record := store_record host_function.
 Let function_closure := function_closure host_function.
-(*Let administrative_instruction := administrative_instruction host_function.
-
-Let to_e_list : seq basic_instruction -> seq administrative_instruction := @to_e_list _.
-Let to_b_list : seq administrative_instruction -> seq basic_instruction := @to_b_list _.*)
 Let e_typing : store_record -> t_context -> seq administrative_instruction -> function_type -> Prop :=
   @e_typing _.
 Let inst_typing : store_record -> instance -> t_context -> bool := @inst_typing _.
-(*Let reduce_simple : seq administrative_instruction -> seq administrative_instruction -> Prop :=
-  @reduce_simple _.
-Let const_list : seq administrative_instruction -> bool := @const_list _.
-Let lholed := lholed host_function.
-Let lfilled : depth -> lholed -> seq administrative_instruction -> seq administrative_instruction -> bool :=
-  @lfilled _.
-Let es_is_basic : seq administrative_instruction -> Prop := @es_is_basic _.*)
 
 Let host := host host_function.
 
@@ -45,6 +34,7 @@ Let s_globals : store_record -> seq global := @s_globals _.
 Let s_mems : store_record -> seq memory := @s_mems _.
 Let functions_agree : seq function_closure -> nat -> function_type -> bool := @functions_agree _.
 Let cl_type : function_closure -> function_type := @cl_type _.
+Let func_extension: function_closure -> function_closure -> bool := @func_extension _.
 Let store_extension: store_record -> store_record -> Prop := @store_extension _.
 
 Definition t_be_value bes : Prop :=
@@ -759,13 +749,7 @@ Proof.
     apply bet_weakening.
     by eapply IHHType => //=.
 Qed.
- (*
-Ltac invert_non_be:=
-  repeat lazymatch goal with
-  | H: exists e, _ = AI_basic e |- _ =>
-    try by destruct H
-  end.
-*)
+
 (*
   Preservation for all be_typeable simple reductions.
 *)
@@ -1054,40 +1038,6 @@ Proof.
     by exists ts, ts2.
 Qed.
 
-(*
-  Looking at what we want to prove in the Lfilled_break case, it might be tempting to
-    prove the following:
-
-Lemma Lfilled_break_typing: forall n lh vs LI ts s C t2s,
-    e_typing s (upd_label C ([::ts] ++ tc_label C)) LI (Tf [::] t2s) ->
-    const_list vs ->
-    length ts = length vs ->
-    lfilled n lh (vs ++ [::AI_basic (Br n)]) LI ->
-    e_typing s C vs (Tf [::] ts).
-
-  The lemma itself is definitely correct, and an apparent approach is to do induction
-    on n (or induction on the lfilled hypothesis).
-
-  However, this will *NOT* work: the culprit is that there is no inductive relationship
-    that changes the instruction (Br n+1) into (Br n), and we will get a useless
-    induction hypothesis that can never be applied.
-
-  We need to somehow avoid getting the parameter of Br into induction. By the lfilled
-    hypothesis, we know LI is a nested Label which, at the innermost level, has (Br n)
-    as its first non-constant instruction, and vs at the top of the value stack.
-
-  Recall that (Br n) looks at the nth entry in the label of the typing context and
-    needs to consume that type. Since we can only induct on the depth of lfilled
-    (but not the n in the instruction), they have to be two separate numbers, say
-    n and m. Now if n is 0, the instruction will basically look at the mth entry;
-    what if n is not 0? In that case if we trace the expansion of LI and simulate
-    how the typing is evaluated, we realize that there will be n entries prepended
-    to the label of the typing context, after which we'll then find the mth element
-    of it due to the (Br m).
-
-  So a more sensible lemma to prove is the following, which the original lemma we
-    wanted is a special case of:
-*)
 
 Lemma Lfilled_break_typing: forall n m k lh vs LI ts s C t2s tss,
     e_typing s (upd_label C (tss ++ [::ts] ++ tc_label C)) LI (Tf [::] t2s) ->
@@ -1168,72 +1118,6 @@ Proof.
     by lias.
 Qed.
 
-(*
-  And yes, the above observation was obviously the result of some futile attempt
-    to prove the unprovable version of the lemma.
-
-Lemma Lfilled_break_typing: forall n lh vs LI ts s C t2s,
-    e_typing s (upd_label C ([::ts] ++ tc_label C)) LI (Tf [::] t2s) ->
-    const_list vs ->
-    length ts = length vs ->
-    lfilled n lh (vs ++ [::AI_basic (Br n)]) LI ->
-    e_typing s C vs (Tf [::] ts).
-Proof.
-  move => n lh vs LI ts s C ts2 HType HConst HLength HLF.
-  apply const_es_exists in HConst. destruct HConst. subst.
-  move/lfilledP in HLF.
-  generalize dependent ts2.
-  generalize dependent LI.
-  induction n.
-  - move => LI HLF ts2 HType.
-    repeat rewrite catA in HType.
-    inversion HLF.
-    apply const_es_exists in H. destruct H. subst.
-    apply e_composition_typing in HType.
-    destruct HType as [ts0 [t1s [t2s [t3s [H1 [H2 [H3 H4]]]]]]].
-    destruct ts0 => //=.
-    destruct t1s => //=.
-    subst. clear H1.
-    apply e_composition_typing in H4.
-    destruct H4 as [ts0' [t1s' [t2s' [t3s' [H5 [H6 [H7 H8]]]]]]].
-    subst.
-    apply e_composition_typing in H7.
-    destruct H7 as [ts0'' [t1s'' [t2s'' [t3s'' [H9 [H10 [H11 H12]]]]]]].
-    subst.
-    apply et_to_bet in H12; last by auto_basic.
-    apply Break_typing in H12.
-    destruct H12 as [ts0 [ts1 [H13 [H14 H15]]]]. clear H13.
-    unfold plop2 in H14. simpl in H14. move/eqP in H14. inversion H14. subst.
-    clear H14.
-    apply et_to_bet in H11; last by (apply const_list_is_basic; apply v_to_e_is_const_list).
-    apply Const_list_typing in H11.
-    repeat rewrite length_is_size in HLength.
-    assert ((ts1 == t1s'') && (ts0 == vs_to_vts x)).
-    + apply concat_cancel_last_n => //=. rewrite size_map.
-      by rewrite v_to_e_size in HLength.
-    + move/andP in H. destruct H.
-      move/eqP in H0. subst.
-      apply ety_a'; first by apply const_list_is_basic; apply v_to_e_is_const_list.
-      by apply Const_list_typing_empty.
-  - move => LI HLF ts2 HType.
-    inversion HLF. subst.
-    repeat rewrite catA in HType.
-    apply e_composition_typing in HType.
-    destruct HType as [ts0 [t1s [t2s [t3s [H2 [H3 [H4 H5]]]]]]].
-    destruct ts0 => //=.
-    destruct t1s => //=.
-    clear H2. clear H3.
-    apply e_composition_typing in H4.
-    destruct H4 as [ts0' [t1s' [t2s' [t3s' [H6 [H7 [H8 H9]]]]]]].
-    destruct ts0' => //=.
-    destruct t1s' => //=.
-    clear H6. clear H7.
-    apply Label_typing in H9.
-    destruct H9 as [ts0'' [t2s'' [H10 [H11 [H12 H13]]]]]. subst.
-    simpl in H12.
-
- *)
-
 Lemma Local_typing: forall s C n f es t1s t2s,
     e_typing s C [::AI_local n f es] (Tf t1s t2s) ->
     exists ts, t2s = t1s ++ ts /\
@@ -1283,16 +1167,6 @@ Proof.
     split => //=.
     by rewrite -catA.
 Qed.
-
-(*
-  Similarly, Local does not involve in induction either. So what we want to prove
-    is also slightly different from what we desire. However, this one is easier
-    to observe.
-
-  The only thing that got me stuck for a while is to observe that label of the
-    typing context plays no role in typing for this case; this is required since
-    we'll get an extra label update from inverting the Label instruction.
- *)
 
 Lemma Lfilled_return_typing: forall n lh vs LI ts s C lab t2s,
     e_typing s (upd_label C lab) LI (Tf [::] t2s) ->
@@ -1462,30 +1336,6 @@ Proof.
          unfold vs_to_vts. rewrite size_map.
          by rewrite v_to_e_size.
   - (* Label_const *)
- (*   Check HType.
-    dependent induction HType.
-    Print e_typing.
-    gen_ind_pre HType.
-    Set Ltac Debug.
-    Check Datatypes.cons.
-    gen_ind_gen HType.
-    gen_ind_subst HType.*)
- (* After several futile attempts to fix gen_ind_gen, I gave up on it and 
-      made a more cumbersome et_dependent_ind that only works for e_typing.
-
-    For future reference: the reason gen_ind_gen fails here is because when we get to
-      the second last term 
-          [::Label n es0 es'] 
-      which is effectively
-          cons (Label n es0 es') nil
-      we first try to generalize the token 'cons', which obviously cannot be 
-        generalized (which is fine); but then when we try to look at the term 'Label',
-        the tactic somehow wants to generalize on the type of it, i.e.
-          'administrative_instruction', 
-        which is unfortunately redefined with host to be 
-          'administrative_instruction host_function'
-        which means we will generalize host_function which is what we tried to avoid.
- *)
     et_dependent_ind HType => //.
     + (* ety_a *)
       assert (es_is_basic (operations.to_e_list bes)); first by apply to_e_list_basic.
@@ -1974,6 +1824,7 @@ Proof.
   destruct g0 => //=.
   destruct g1 => //=.
   simpl in H2. simpl in H1.
+  remove_bools_options; subst; first by rewrite H0; lias.
   by destruct g_mut => //=; remove_bools_options;
     apply/andP => //=; subst; split => //=;
     destruct g_mut0 => //=; destruct g_val => //=; destruct g_val0 => //=.
@@ -1981,125 +1832,129 @@ Qed.
 
 Lemma glob_extension_C: forall sg sg' ig tcg,
     all2 (globals_agree sg) ig tcg ->
-    all2 glob_extension sg sg' ->
+    comp_extension sg sg' glob_extension ->
     all2 (globals_agree sg') ig tcg.
 Proof.
-  move => sg sg' ig.
-  generalize dependent sg; generalize dependent sg'.
-  induction ig; move => sg' sg tcg HA Hext => //=; destruct tcg => //=.
-  - simpl in HA. remove_bools_options.
-    edestruct IHig; eauto.
-    unfold globals_agree in H. remove_bools_options.
-    assert (size sg = size sg'); first by eapply all2_size; eauto.
-    assert (a < length sg')%coq_nat.
-    {
-        rewrite length_is_size in H. rewrite length_is_size.
-        rewrite -H1. by lias.
-    }
-    remember H2 as H5. clear HeqH5.
-    rewrite <- List.nth_error_Some in H2.
-    destruct (List.nth_error sg' a) eqn:HGlob => //=; eauto. clear H2.
-    remember Hext as Hext1. clear HeqHext1.
-    eapply all2_projection in Hext1; eauto.
-    apply/andP. split => //=.
-    + unfold globals_agree. apply/andP; split => //=; first by lias.
-      unfold option_map. rewrite HGlob.
-      apply/eqP. f_equal.
-      by eapply global_agree_extension; eauto.
-    + by eapply IHig; eauto.
+  move => sg sg' ig tcg Hagree Hext.
+  eapply all2_weaken; try apply Hagree.
+  move => x y Hgagree.
+  unfold globals_agree in *.
+  unfold comp_extension in Hext.
+  remove_bools_options.
+  destruct (List.nth_error sg' x) as [g' |] eqn:Hnth; last by apply List.nth_error_None in Hnth; lias.
+  simpl in *.
+  apply (nth_error_take (k := length sg)) in Hnth => //.
+  apply/andP; split; first by lias.
+  specialize (all2_projection H2 Hoption Hnth) as Hproj.
+  eapply global_agree_extension in Hproj; last by apply H4.
+  by apply/eqP; f_equal; lias.
 Qed.
 
-Lemma memi_agree_extension: forall m0 m1 n m,
-    memi_agree m0 n m ->
-    all2 mem_extension m0 m1 ->
-    memi_agree m1 n m.
+Lemma mem_typing_extension: forall m m' y,
+    mem_typing m y ->
+    mem_extension m m' ->
+    mem_typing m' y.
 Proof.
-  move => m0 m1 n m H1 H2.
-  assert (size m0 = size m1) as HSize; first by eapply all2_size; eauto.
-  unfold memi_agree.
-  unfold memi_agree in H1. unfold mem_extension in H2.
-  destruct m => //=.
+  move => m m' y Htype Hext.
+  unfold mem_typing in *.
+  unfold mem_extension in Hext.
   remove_bools_options.
-  rewrite length_is_size in H.
-  apply/andP; split => //=; first by rewrite HSize in H.
-  rewrite HSize in H.
-  rewrite -length_is_size in H.
-  move/ltP in H.
-  rewrite <- List.nth_error_Some in H.
-  destruct (List.nth_error m1 n) eqn:HN => //=.
-  unfold mem_typing. simpl.
-  eapply all2_projection in H2; [| by apply Hoption | by apply HN ].
-  unfold mem_typing in H0. simpl in H0.
-  remove_bools_options.
-  apply/andP; split.
-  - apply N.leb_le. apply N.leb_le in H1. apply N.leb_le in H0.
+  apply/andP; split; last by apply/eqP; rewrite -H2 -H0.
+  { apply/N.leb_spec0.
+    move/N.leb_spec0 in H.
+    move/N.leb_spec0 in H1.
     by lias.
-  - rewrite H3 in H2. rewrite H2. by apply/eqP.
+  }
 Qed.
 
 Lemma mem_extension_C: forall sm sm' im tcm,
     all2 (memi_agree sm) im tcm ->
-    all2 mem_extension sm sm' ->
+    comp_extension sm sm' mem_extension ->
     all2 (memi_agree sm') im tcm.
 Proof.
-  move => sm sm' im.
-  generalize dependent sm; generalize dependent sm'.
-  induction im; move => sm' sm tcm HA Hext => //=; destruct tcm => //=.
-  simpl in HA. remove_bools_options.
-  apply/andP; split => //=; last by eapply IHim; eauto.
-  by eapply memi_agree_extension; eauto.
+  move => sm sm' im tcm Hagree Hext.
+  eapply all2_weaken; try apply Hagree.
+  move => x y Hmagree.
+  unfold memi_agree in *.
+  unfold comp_extension in Hext.
+  remove_bools_options.
+  destruct (List.nth_error sm' x) as [m' |] eqn:Hnth; last by apply List.nth_error_None in Hnth; lias.
+  apply (nth_error_take (k := length sm)) in Hnth => //.
+  apply/andP; split; first by lias.
+  specialize (all2_projection H2 Hoption Hnth) as Hproj.
+  by eapply mem_typing_extension; eauto.
 Qed.
 
-Lemma tabi_agree_extension: forall t0 t1 n t,
-    tabi_agree t0 n t ->
-    all2 tab_extension t0 t1 ->
-    tabi_agree t1 n t.
+Lemma tab_typing_extension: forall t t' y,
+    tab_typing t y ->
+    tab_extension t t' ->
+    tab_typing t' y.
 Proof.
-  move => t0 t1 n t H1 H2.
-  assert (size t0 = size t1) as HSize; first by eapply all2_size; eauto.
-  unfold tabi_agree.
-  unfold tabi_agree in H1. unfold tab_extension in H2.
-  unfold tab_size in H2.
-  destruct t => //=.
-  destruct t0 => //=.
-  destruct t1 => //=.
-  simpl in H2. simpl in H1.
+  move => t t' y Htype Hext.
+  unfold tab_typing in *.
+  unfold tab_extension in Hext.
   remove_bools_options.
-  unfold tab_typing in H3.
-  remove_bools_options.
-  simpl in H3. simpl in H4.
-  unfold tab_typing. simpl.
-  simpl in HSize. inversion HSize. subst. clear HSize.
-  apply/andP; split => //=.
-  - rewrite length_is_size in H1. rewrite length_is_size. by rewrite H6 in H1.
-  - assert (List.nth_error (t1 :: t2) n <> None).
-    { apply List.nth_error_Some. rewrite length_is_size. simpl. rewrite -H6.
-      by lias. }
-    destruct (List.nth_error (t1 :: t2) n) eqn:HN => //=.
-    destruct n => //=.
-    + simpl in HN. simpl in Hoption. inversion HN. inversion Hoption. subst.
-      apply/andP; split => //=; last by rewrite -H2.
-      unfold tab_size. unfold tab_size in H3. by lias.
-    + simpl in HN. simpl in Hoption.
-      eapply all2_projection in H0; eauto.
-      remove_bools_options.
-      apply/andP; split => //=; last by rewrite -H7.
-      unfold tab_size. unfold tab_size in H3. by lias.
+  apply/andP; split; last by apply/eqP; rewrite -H0; lias.
+  by lias.
 Qed.
 
 Lemma tab_extension_C: forall st st' it tct,
     all2 (tabi_agree st) it tct ->
-    all2 tab_extension st st' ->
+    comp_extension st st' tab_extension ->
     all2 (tabi_agree st') it tct.
 Proof.
-  move => st st' it.
-  generalize dependent st; generalize dependent st'.
-  induction it; move => st' st tct HA Hext => //=; destruct tct => //=.
-  simpl in HA. remove_bools_options.
-  apply/andP; split => //=; last by eapply IHit; eauto.
-  by eapply tabi_agree_extension; eauto.
+  move => st st' it tct Hagree Hext.
+  eapply all2_weaken; try apply Hagree.
+  move => x y Htagree.
+  unfold tabi_agree in *.
+  unfold comp_extension in Hext.
+  remove_bools_options.
+  destruct (List.nth_error st' x) as [t' |] eqn:Hnth; last by apply List.nth_error_None in Hnth; lias.
+  apply (nth_error_take (k := length st)) in Hnth => //.
+  apply/andP; split; first by lias.
+  specialize (all2_projection H2 Hoption Hnth) as Hproj.
+  by eapply tab_typing_extension; eauto.
 Qed.
 
+Lemma func_agree_extension: forall f0 f1 n f,
+    typing.functions_agree f0 n f ->
+    comp_extension f0 f1 func_extension ->
+    typing.functions_agree f1 n f.
+Proof.
+  move => f0 f1 n f Hagree Hext.
+  unfold comp_extension, func_extension, operations.func_extension in Hext.
+  unfold typing.functions_agree in *.
+  remove_bools_options.
+  apply/andP; split; first lias.
+  assert (List.nth_error f1 n = Some f2) as Hnth; last by rewrite Hnth.
+  assert (f1 = (take (length f0) f1) ++ (drop (length f0) f1)) as Hcat; first by rewrite cat_take_drop.
+  rewrite -> Hcat.
+  remember (take (length f0) f1) as f0'.
+  assert (f0 = f0') as ->.
+  { clear - H0. move : f0' H0.
+    induction f0; move => f0' H0; destruct f0' => //=.
+    simpl in *.
+    remove_bools_options; subst.
+    f_equal.
+    by apply IHf0.
+  }
+  rewrite List.nth_error_app1 => //.
+  by lias.
+Qed.
+  
+Lemma func_extension_C: forall sf sf' fi tcf,
+    all2 (typing.functions_agree sf) fi tcf ->
+    comp_extension sf sf' func_extension ->
+    all2 (typing.functions_agree sf') fi tcf.
+Proof.
+  move => sf sf' fi.
+  move: sf sf'.
+  induction fi; move => sf sf' tcf HA Hext => //=; destruct tcf => //=.
+  simpl in HA. remove_bools_options.
+  apply/andP; split => //=; last by eapply IHfi; eauto.
+  by eapply func_agree_extension; eauto.
+Qed.
+  
 Lemma inst_typing_extension: forall s s' i C,
     store_extension s s' ->
     inst_typing s i C ->
@@ -2112,12 +1967,14 @@ Proof.
   destruct i => //=.
   destruct C => //=.
   destruct tc_local => //. destruct tc_label => //. destruct tc_return => //.
-  remove_bools_options. rewrite - H4.
+  remove_bools_options. 
   repeat (apply/andP; split => //=; subst => //=).
+  - by eapply func_extension_C; eauto.
   - by eapply glob_extension_C; eauto.
   - by eapply tab_extension_C; eauto.
   - by eapply mem_extension_C; eauto.
 Qed.
+
 
 Lemma frame_typing_extension: forall s s' f C,
     store_extension s s' ->
@@ -2141,6 +1998,14 @@ Proof.
   by apply IHl.
 Qed.
 
+Lemma all2_func_extension_same: forall f,
+    all2 func_extension f f.
+Proof.
+  move => f.
+  apply reflexive_all2_same. unfold reflexive. move => x. unfold func_extension, operations.func_extension.
+  by apply/eqP.
+Qed.
+
 Lemma all2_tab_extension_same: forall t,
     all2 tab_extension t t.
 Proof.
@@ -2158,13 +2023,21 @@ Proof.
   by apply N.leb_le; lias.
 Qed.
 
+Lemma glob_extension_refl: forall t,
+    glob_extension t t.
+Proof.
+  move => t.
+  unfold glob_extension.
+  do 2 (apply/andP; split => //).
+  apply/orP.
+  by right.
+Qed.
+
 Lemma all2_glob_extension_same: forall t,
     all2 glob_extension t t.
 Proof.
   move => t.
-  apply reflexive_all2_same. unfold reflexive. move => x. unfold glob_extension.
-  destruct (g_mut x) => //=.
-  by destruct (g_val x).
+  apply reflexive_all2_same. unfold reflexive. by apply glob_extension_refl.
 Qed.
 
 Ltac convert_et_to_bet:=
@@ -2249,30 +2122,31 @@ Lemma store_extension_same: forall s,
     store_extension s s.
 Proof.
   move => s. unfold store_extension.
-  repeat (apply/andP; split).
-  + by apply/eqP.
+  repeat (apply/andP; split => //); rewrite length_is_size take_size.
+  + by apply all2_func_extension_same.
   + by apply all2_tab_extension_same.
   + by apply all2_mem_extension_same.
   + by apply all2_glob_extension_same.
 Qed.
 
-(* This is the only questionable lemma that I'm not >99% sure of it's correctness.
-   But it seems to be absolutely required. Maybe I'm 98% sure. *)
-(*
-   UPD: oops, this is in fact completely nonsense and in no way required --
-          I overlooked another possibility here. This is now abandoned and
-          replaced by a correct version.
-
-Lemma store_reduce_same_es_typing: forall s vs es i s' vs' es' es0 C C' loc lab ret tf,
-    reduce s vs es i s' vs' es' ->
-    store_typing s ->
-    store_typing s' ->
-    inst_typing s i C ->
-    inst_typing s' i C' ->
-    e_typing s (upd_label (upd_local_return C loc ret) lab) es0 tf ->
-    e_typing s' (upd_label (upd_local_return C' loc ret) lab) es0 tf.
+Lemma store_extension_lookup: forall s s' n cl,
+    store_extension s s' ->
+    List.nth_error (s_funcs s) n = Some cl ->
+    List.nth_error (s_funcs s') n = Some cl.
 Proof.
- *)
+  move => s s' n cl Hext Hnth.
+  unfold store_extension, operations.store_extension in Hext.
+  remove_bools_options.
+  clear H0 H1 H2.
+  unfold comp_extension in H.  
+  remove_bools_options.
+  assert (lt n (length (s_funcs s))) as Hlen; first by apply List.nth_error_Some; rewrite Hnth.
+  destruct (List.nth_error (s_funcs s') n) as [cl' |] eqn:Hnth'; last by apply List.nth_error_None in Hnth'; lias.
+  apply (nth_error_take (k := length (s_funcs s))) in Hnth'; last by lias.
+  specialize (all2_projection H0 Hnth Hnth') as Hproj.
+  unfold operations.func_extension in Hproj.
+  by move/eqP in Hproj; subst.
+Qed.
 
 Lemma store_extension_cl_typing: forall s s' cl tf,
     store_extension s s' ->
@@ -2285,11 +2159,6 @@ Proof.
     by eapply inst_typing_extension; eauto.
   - by eapply cl_typing_host; eauto.
 Qed.
-
-(*
-  The correct version. We need a mutual induction on e_typing and s_typing
-    since they were defined with a mutual induction.
- *)
 
 Lemma store_extension_e_typing: forall s s' C es tf,
     store_typing s ->
@@ -2325,11 +2194,8 @@ Proof.
     apply ety_local => //.
     by eapply IHHType; try apply HST1 => //.
   - move=> s a C cl tf HNth HCLType s' HST1 HST2 Hext.
-    replace (s_funcs s) with (s_funcs s') in HNth.
-    eapply ety_invoke; eauto => //.
+    eapply ety_invoke; eauto => //; first by eapply store_extension_lookup; eauto.
     by eapply store_extension_cl_typing; eauto.
-    { unfold store_extension, operations.store_extension in Hext.
-      by remove_bools_options. }  
   - move=> s C es es' t1s t2s n HType1 IHHType1 HType2 IHHType2 E s' HST1 HST2 Hext.
     eapply ety_label => //; eauto.
     + by apply IHHType1.
@@ -2355,7 +2221,7 @@ Proof.
     rewrite -update_list_at_is_set_nth; last by lias.
     simpl.
     apply/andP. split.
-    + unfold glob_extension. destruct (g_mut g0) => //=. by destruct (g_val g0).
+    + by apply glob_extension_refl. 
     + rewrite update_list_at_is_set_nth.
       * by eapply IHn; eauto.
       * simpl in H. rewrite length_is_size in H. by lias.
@@ -2814,6 +2680,33 @@ Proof.
   by induction HReduce.
 Qed.
 
+Lemma store_extension_mem: forall s i mem mem',
+  List.nth_error s.(s_mems) i = Some mem ->
+  mem_extension mem mem' ->
+  store_extension s (upd_s_mem s (update_list_at (s_mems s) i mem')).
+Proof.
+  move => s i mem mem' Hnth Hext.
+  unfold store_extension => //=.
+  repeat (apply/andP; split) => //=.
+  - by rewrite length_is_size take_size; apply all2_func_extension_same.
+  - by rewrite length_is_size take_size; apply all2_tab_extension_same.
+  - rewrite update_list_at_length => //.
+    by apply/ltP; rewrite - List.nth_error_Some; rewrite Hnth.
+  - match goal with
+    | |- context [take ?n ?l] => remember l as l'
+    | _ => idtac
+    end.
+    assert (length l' = length s.(s_mems)) as Hlen.
+    { subst l'; apply update_list_at_length.
+      by apply/ltP; rewrite - List.nth_error_Some; rewrite Hnth.
+    }
+    rewrite - Hlen.
+    rewrite length_is_size take_size.
+    subst l'.
+    eapply mem_extension_update_nth; eauto => //=.
+  - by rewrite length_is_size take_size; apply all2_glob_extension_same.
+Qed. 
+
 Lemma store_extension_reduce: forall s f es s' f' es' C tf loc lab ret hs hs',
     reduce hs s f es hs' s' f' es' ->
     inst_typing s f.(f_inst) C ->
@@ -2853,13 +2746,27 @@ Proof.
     unfold is_mut in H7. simpl in H7. remove_bools_options. subst.
     + simpl. unfold store_extension => //=.
       repeat (apply/andP; split) => //=.
-      -- by apply all2_tab_extension_same.
-      -- by apply all2_mem_extension_same.
-      -- eapply glob_extension_update_nth; eauto => //=.
+      -- by rewrite length_is_size take_size; apply all2_func_extension_same.
+      -- by rewrite length_is_size take_size; apply all2_tab_extension_same.
+      -- by rewrite length_is_size take_size; apply all2_mem_extension_same.
+      -- rewrite update_list_at_length => //.
+         by apply/ltP; rewrite - List.nth_error_Some; rewrite Hoption0.
+      -- match goal with
+         | |- context [take ?n ?l] => remember l as l'
+         | _ => idtac
+         end.
+         assert (length l' = length s.(s_globals)) as Hlen.
+         { subst l'; apply update_list_at_length.
+           by apply/ltP; rewrite - List.nth_error_Some; rewrite Hoption0.
+         }
+         rewrite - Hlen.
+         rewrite length_is_size take_size.
+         subst l'.
+         eapply glob_extension_update_nth; eauto => //=.
          unfold glob_extension => //=.
          by destruct v => //=; destruct g_val => //=.
-    split => //.
-    by eapply store_global_extension_store_typed; eauto;
+      split => //.
+      by eapply store_global_extension_store_typed; eauto;
       destruct s => //=; destruct s' => //=; remove_bools_options.
   - (* update memory : store none *)
     apply et_to_bet in HType; auto_basic. simpl in HType.
@@ -2873,12 +2780,9 @@ Proof.
     remove_bools_options.
     inversion H4. subst. clear H4.
     assert (store_extension s (upd_s_mem s (update_list_at (s_mems s) i mem'))) as Hext.
-    + unfold store_extension => //=.
-      repeat (apply/andP; split) => //=.
-      * by apply all2_tab_extension_same.
-        eapply mem_extension_update_nth; eauto => //=.
-      * by eapply mem_extension_store; eauto.
-      * by apply all2_glob_extension_same.
+    { eapply store_extension_mem => //; first by rewrite H1.
+      by eapply mem_extension_store; eauto.
+    }
     split => //.
     eapply store_memory_extension_store_typed; eauto => //=.
     remember HST as HST2. clear HeqHST2.
@@ -2905,12 +2809,9 @@ Proof.
     remove_bools_options.
     inversion H4. subst. clear H4.
     assert (store_extension s (upd_s_mem s (update_list_at (s_mems s) i mem'))) as Hext.
-    + unfold store_extension => //=.
-      repeat (apply/andP; split) => //=.
-      * by apply all2_tab_extension_same.
-      * eapply mem_extension_update_nth; eauto => //=.
-        by eapply mem_extension_store; eauto.
-      * by apply all2_glob_extension_same.
+    { eapply store_extension_mem => //; first by rewrite H1.
+      by eapply mem_extension_store; eauto.
+    }
     split => //.
     eapply store_memory_extension_store_typed; eauto => //=.
     remember HST as HST2. clear HeqHST2.
@@ -2934,12 +2835,9 @@ Proof.
     destruct H6 as [ts' [H7 [H8 H9]]]. subst.
     apply concat_cancel_last in H9 => //. destruct H9. subst.
     assert (store_extension s (upd_s_mem s (update_list_at (s_mems s) i mem'))) as Hext.
-    + unfold store_extension => //=.
-      repeat (apply/andP; split) => //=.
-      * by apply all2_tab_extension_same.
-      * eapply mem_extension_update_nth; eauto => //=.
-        by eapply mem_extension_grow_memory; eauto.
-      * by apply all2_glob_extension_same.
+    { eapply store_extension_mem => //; first by rewrite H0.
+      by eapply mem_extension_grow_memory; eauto.
+    }
     split => //.
     eapply store_memory_extension_store_typed; eauto => //=.
     remember HST as HST2. clear HeqHST2.
